theories/lang/cpp/logic/stmt.v
@@ -21,18 +21,18 @@ Module Type Stmt.
    *)
   Section with_resolver.
     Context `{Σ : cpp_logic thread_info} {resolve:genv}.
-    Variables (M : coPset) (ti : thread_info) (ρ : region).
+    Variables (M : coPset) (ti : thread_info).
 
-    Local Notation wp := (wp (resolve:=resolve) M ti ρ).
-    Local Notation wpe := (wpe (resolve:=resolve) M ti ρ).
-    Local Notation wp_lval := (wp_lval (resolve:=resolve) M ti ρ).
-    Local Notation wp_prval := (wp_prval (resolve:=resolve) M ti ρ).
-    Local Notation wp_xval := (wp_xval (resolve:=resolve) M ti ρ).
-    Local Notation wp_glval := (wp_glval (resolve:=resolve) M ti ρ).
-    Local Notation wp_rval := (wp_rval (resolve:=resolve) M ti ρ).
-    Local Notation wp_init := (wp_init (resolve:=resolve) M ti ρ).
-    Local Notation wpAny := (wpAny (resolve:=resolve) M ti ρ).
-    Local Notation wpAnys := (wpAnys (resolve:=resolve) M ti ρ).
+    Local Notation wp := (wp (resolve:=resolve) M ti).
+    Local Notation wpe := (wpe (resolve:=resolve) M ti).
+    Local Notation wp_lval := (wp_lval (resolve:=resolve) M ti).
+    Local Notation wp_prval := (wp_prval (resolve:=resolve) M ti).
+    Local Notation wp_xval := (wp_xval (resolve:=resolve) M ti).
+    Local Notation wp_glval := (wp_glval (resolve:=resolve) M ti).
+    Local Notation wp_rval := (wp_rval (resolve:=resolve) M ti).
+    Local Notation wp_init := (wp_init (resolve:=resolve) M ti).
+    Local Notation wpAny := (wpAny (resolve:=resolve) M ti).
+    Local Notation wpAnys := (wpAnys (resolve:=resolve) M ti).
     Local Notation fspec := (fspec ti).
     Local Notation mdestroy := (@mdestroy Σ resolve ti) (only parsing).
     Local Notation destruct := (destruct (σ:=resolve) ti) (only parsing).
@@ -55,10 +55,10 @@ Module Type Stmt.
    (* the semantics of return is like an initialization
      * expression.
      *)
-    Axiom wp_return_void : forall Q,
-        Q.(k_return) None empSP |-- wp (Sreturn None) Q.
+    Axiom wp_return_void : forall ρ Q,
+        Q.(k_return) None empSP |-- wp ρ (Sreturn None) Q.
 
-    Axiom wp_return : forall c e Q,
+    Axiom wp_return : forall ρ c e Q,
         (if is_aggregate (type_of e) then
            (* ^ C++ erases the reference information on types for an unknown
             * reason, see http://eel.is/c++draft/expr.prop#expr.type-1.sentence-1
@@ -67,31 +67,31 @@ Module Type Stmt.
             *)
            match c with
            | Rvalue =>
-             Exists a, result_addr ρ a ** ltrue //\\
-             wp_init (erase_qualifiers (type_of e)) (Vptr a) (not_mine e) (Q.(k_return) (Some (Vptr a)))
+             Exists a, _result ρ &~ a ** ltrue //\\
+             wp_init ρ (erase_qualifiers (type_of e)) (Vptr a) (not_mine e) (Q.(k_return) (Some (Vptr a)))
            | Lvalue
            | Xvalue =>
-             wpe c e (fun v => Q.(k_return) (Some v))
+             wpe ρ c e (fun v => Q.(k_return) (Some v))
            end
          else
-           wpe c e (fun v => Q.(k_return) (Some v)))
-        |-- wp (Sreturn (Some (c, e))) Q.
+           wpe ρ c e (fun v => Q.(k_return) (Some v)))
+        |-- wp ρ (Sreturn (Some (c, e))) Q.
 
-    Axiom wp_break : forall Q,
-        |> Q.(k_break) |-- wp Sbreak Q.
-    Axiom wp_continue : forall Q,
-        |> Q.(k_continue) |-- wp Scontinue Q.
+    Axiom wp_break : forall ρ Q,
+        |> Q.(k_break) |-- wp ρ Sbreak Q.
+    Axiom wp_continue : forall ρ Q,
+        |> Q.(k_continue) |-- wp ρ Scontinue Q.
 
-    Axiom wp_expr : forall vc e Q,
-        |> wpAny (vc,e) (SP (fun _ => Q.(k_normal)))
-        |-- wp (Sexpr vc e) Q.
+    Axiom wp_expr : forall ρ vc e Q,
+        |> wpAny ρ (vc,e) (SP (fun _ => Q.(k_normal)))
+        |-- wp ρ (Sexpr vc e) Q.
 
     (* This definition performs allocation of local variables
      * note that references do not allocate anything in the semantics, they are
      * just aliases.
      *)
-    Fixpoint wp_decl (x : ident) (ty : type) (init : option Expr) (dtor : option obj_name)
-               (k : Kpreds -> mpred) (Q : Kpreds)
+    Fixpoint wp_decl (ρ : region) (x : ident) (ty : type) (init : option Expr) (dtor : option obj_name)
+               (k : region -> Kpreds -> mpred) (Q : Kpreds)
                (* ^ Q is the continuation for after the declaration
                 *   goes out of scope.
                 * ^ k is the rest of the declaration
@@ -108,14 +108,14 @@ Module Type Stmt.
       | Tint _ _ =>
         Forall a : ptr,
         let done :=
-            k (Kfree (tlocal_at ρ x a (anyR (erase_qualifiers ty) 1)) Q)
+            k (Rbind x a ρ) (Kfree (_at (_eq a) (anyR (erase_qualifiers ty) 1)) Q)
         in
-        let continue := local_addr ρ x a -* done in
+        let continue := done in
         match init with
         | None =>
           _at (_eq a) (uninitR (erase_qualifiers ty) 1) -* continue
         | Some init =>
-          wp_prval init (fun v free => free **
+          wp_prval ρ init (fun v free => free **
                               _at (_eq a) (primR (erase_qualifiers ty) 1 v) -* continue)
         end
 
@@ -128,12 +128,12 @@ Module Type Stmt.
                       end (_at (_eq a) (anyR (erase_qualifiers ty) 1))
                   in
                   let continue :=
-                      local_addr ρ x a -* k (Kfree (local_addr ρ x a ** destroy) Q)
+                      k (Rbind x a ρ) (Kfree destroy Q)
                   in
                   match init with
                   | None => continue
                   | Some init =>
-                    wp_init ty (Vptr a) (not_mine init) (fun free => free ** continue)
+                    wp_init ρ ty (Vptr a) (not_mine init) (fun free => free ** continue)
                   end
       | Tarray ty' N =>
         Forall a, _at (_eq a) (uninitR (erase_qualifiers ty) 1) -*
@@ -144,13 +144,12 @@ Module Type Stmt.
                       end (_at (_eq a) (anyR (erase_qualifiers ty) 1))
                   in
                   let continue :=
-                      local_addr ρ x a -*
-                      k (Kfree (local_addr ρ x a ** _at (_eq a) (anyR (erase_qualifiers ty) 1)) Q)
+                      k (Rbind x a ρ) (Kfree (_at (_eq a) (anyR (erase_qualifiers ty) 1)) Q)
                   in
                   match init with
                   | None => continue
                   | Some init =>
-                    wp_init ty (Vptr a) (not_mine init) (fun free => free ** continue)
+                    wp_init ρ ty (Vptr a) (not_mine init) (fun free => free ** continue)
                   end
 
         (* references *)
@@ -161,109 +160,109 @@ Module Type Stmt.
           (* ^ references must be initialized *)
         | Some init =>
           (* i should use the type here *)
-          wp_lval init (fun a free =>
+          wp_lval ρ init (fun a free =>
              Exists p, [| a = Vptr p |] **
-             local_addr ρ x p -* (free ** k (Kfree (local_addr ρ x p) Q)))
+             (free ** k (Rbind x p ρ) Q))
         end
 
       | Tfunction _ _ => lfalse (* not supported *)
 
-      | Tqualified _ ty => wp_decl x ty init dtor k Q
+      | Tqualified _ ty => wp_decl ρ x ty init dtor k Q
       | Tnullptr =>
         Forall a : ptr,
         let done :=
-            k (Kfree (tlocal_at ρ x a (anyR (erase_qualifiers ty) 1)) Q)
+            k (Rbind x a ρ) (Kfree (_at (_eq a) (anyR (erase_qualifiers ty) 1)) Q)
         in
-        let continue := local_addr ρ x a -* done in
+        let continue := done in
         match init with
         | None =>
           _at (_eq a) (primR Tnullptr 1 (Vptr nullptr)) -* continue
         | Some init =>
-          wp_prval init (fun v free => free **
+          wp_prval ρ init (fun v free => free **
                               _at (_eq a) (primR (erase_qualifiers ty) 1 v) -* continue)
         end
       | Tfloat _ => lfalse (* not supportd *)
       | Tarch _ _ => lfalse (* not supported *)
       end.
 
-    Fixpoint wp_decls (ds : list VarDecl)
-             (k : Kpreds -> mpred) (Q : Kpreds) : mpred :=
+    Fixpoint wp_decls (ρ : region) (ds : list VarDecl)
+             (k : region -> Kpreds -> mpred) (Q : Kpreds) : mpred :=
       match ds with
-      | nil => k Q
+      | nil => k ρ Q
       | {| vd_name := x ; vd_type := ty ; vd_init := init ; vd_dtor := dtor |} :: ds =>
-        |> wp_decl x ty init dtor (wp_decls ds k) Q
+        |> wp_decl ρ x ty init dtor (fun ρ => wp_decls ρ ds k) Q
       end.
 
     (* note(gmm): this rule is non-compositional because
      * wp_decls requires the rest of the block computation
      *)
-    Fixpoint wp_block (ss : list Stmt) (Q : Kpreds) : mpred :=
+    Fixpoint wp_block (ρ : region) (ss : list Stmt) (Q : Kpreds) : mpred :=
       match ss with
       | nil => Q.(k_normal)
       | Sdecl ds :: ss =>
-        wp_decls ds (wp_block ss) Q
+        wp_decls ρ ds (fun ρ => wp_block ρ ss) Q
       | s :: ss =>
-        |> wp s (Kseq (wp_block ss) Q)
+        |> wp ρ s (Kseq (wp_block ρ ss) Q)
       end.
 
-    Axiom wp_seq : forall Q ss,
-        wp_block ss Q |-- wp (Sseq ss) Q.
+    Axiom wp_seq : forall ρ Q ss,
+        wp_block ρ ss Q |-- wp ρ (Sseq ss) Q.
 
-    Axiom wp_if : forall e thn els Q,
-        |> wp_prval e (fun v free =>
+    Axiom wp_if : forall ρ e thn els Q,
+        |> wp_prval ρ e (fun v free =>
              match is_true v with
              | None => lfalse
              | Some c =>
                free **
-                    if c then
-                      wp thn Q
-                    else
-                      wp els Q
+               if c then
+                 wp ρ thn Q
+               else
+                 wp ρ els Q
              end)
-           |-- wp (Sif None e thn els) Q.
+      |-- wp ρ (Sif None e thn els) Q.
 
-    Axiom wp_if_decl : forall d e thn els Q,
-        wp (Sseq (Sdecl (d :: nil) :: Sif None e thn els :: nil)) Q
-        |-- wp (Sif (Some d) e thn els) Q.
+    Axiom wp_if_decl : forall ρ d e thn els Q,
+        wp ρ (Sseq (Sdecl (d :: nil) :: Sif None e thn els :: nil)) Q
+        |-- wp ρ (Sif (Some d) e thn els) Q.
 
     (* note(gmm): this rule is not sound for a total hoare logic
      *)
-    Axiom wp_while : forall t b Q I,
-        I |-- wp (Sif None t (Sseq (b :: Scontinue :: nil)) Sskip)
+    Axiom wp_while : forall ρ t b Q I,
+        I |-- wp ρ (Sif None t (Sseq (b :: Scontinue :: nil)) Sskip)
                 (Kloop I Q) ->
-        I |-- wp (Swhile None t b) Q.
+        I |-- wp ρ (Swhile None t b) Q.
 
-    Axiom wp_while_decl : forall d t b Q,
-        wp (Sseq (Sdecl (d :: nil) :: Swhile None t b :: nil)) Q
-        |-- wp (Swhile (Some d) t b) Q.
+    Axiom wp_while_decl : forall ρ d t b Q,
+        wp ρ (Sseq (Sdecl (d :: nil) :: Swhile None t b :: nil)) Q
+        |-- wp ρ (Swhile (Some d) t b) Q.
 
 
     (* note(gmm): this rule is not sound for a total hoare logic
      *)
-    Axiom wp_for : forall test incr b Q Inv,
+    Axiom wp_for : forall ρ test incr b Q Inv,
         match test with
         | None =>
-          Inv |-- wp (Sseq (b :: Scontinue :: nil))
+          Inv |-- wp ρ (Sseq (b :: Scontinue :: nil))
               (Kloop match incr with
                      | None => Inv
-                     | Some incr => wpAny incr (fun _ _ => Inv)
+                     | Some incr => wpAny ρ incr (fun _ _ => Inv)
                      end Q)
         | Some test =>
-          Inv |-- wp (Sif None test (Sseq (b :: Scontinue :: nil)) Sskip)
+          Inv |-- wp ρ (Sif None test (Sseq (b :: Scontinue :: nil)) Sskip)
               (Kloop match incr with
                      | None => Inv
-                     | Some incr => wpAny incr (fun _ _ => Inv)
+                     | Some incr => wpAny ρ incr (fun _ _ => Inv)
                      end Q)
         end ->
-        Inv |-- wp (Sfor None test incr b) Q.
+        Inv |-- wp ρ (Sfor None test incr b) Q.
 
-    Axiom wp_for_init : forall init test incr b Q,
-        wp (Sseq (init :: Sfor None test incr b :: nil)) Q
-        |-- wp (Sfor (Some init) test incr b) Q.
+    Axiom wp_for_init : forall ρ init test incr b Q,
+        wp ρ (Sseq (init :: Sfor None test incr b :: nil)) Q
+        |-- wp ρ (Sfor (Some init) test incr b) Q.
 
-    Axiom wp_do : forall t b Q I,
-        I |-- wp (Sseq (b :: (Sif None t Scontinue Sskip) :: nil)) (Kloop I Q) ->
-        I |-- wp (Sdo b t) Q.
+    Axiom wp_do : forall ρ t b Q I,
+        I |-- wp ρ (Sseq (b :: (Sif None t Scontinue Sskip) :: nil)) (Kloop I Q) ->
+        I |-- wp ρ (Sdo b t) Q.
 
     (* compute the [Prop] that is known if this switch branch is taken *)
     Definition wp_switch_branch (v : Z) (s : SwitchBranch) : Prop :=
@@ -296,17 +295,17 @@ Module Type Stmt.
 
 
     (* apply the [wp] calculation to the body of a switch *)
-    Fixpoint wp_switch_block (e : Z) (L : Prop) (ls : list Stmt) (Q : Kpreds) : mpred :=
+    Fixpoint wp_switch_block (ρ : region) (e : Z) (L : Prop) (ls : list Stmt) (Q : Kpreds) : mpred :=
       match ls with
       | Scase sb :: ls =>
         let here := wp_switch_branch e sb in
-        ([| here |] -* wp (Sseq ls) Q) //\\
-        wp_switch_block e (L \/ here) ls Q
+        ([| here |] -* wp ρ (Sseq ls) Q) //\\
+        wp_switch_block ρ e (L \/ here) ls Q
       | Sdefault :: ls =>
-        [| ~L |] -* wp_switch_block e L ls Q
+        [| ~L |] -* wp_switch_block ρ e L ls Q
       | s :: ls =>
         if no_case s then
-          wp_switch_block e L ls Q
+          wp_switch_block ρ e L ls Q
         else
           lfalse
       | nil => lfalse
@@ -321,17 +320,17 @@ Module Type Stmt.
        ; k_break  := k.(k_normal)
        ; k_continue := k.(k_continue) |}.
 
-    Axiom wp_switch : forall e b Q,
-        wp_prval e (fun v free =>
+    Axiom wp_switch : forall ρ e b Q,
+        wp_prval ρ e (fun v free =>
                     Exists vv : Z, [| v = Vint vv |] **
-                    wp_switch_block vv False b (Kswitch Q))
-        |-- wp (Sswitch e (Sseq b)) Q.
+                    wp_switch_block ρ vv False b (Kswitch Q))
+        |-- wp ρ (Sswitch e (Sseq b)) Q.
 
     (* note: case and default statements are only meaningful inside of [switch].
      * this is handled by [wp_switch_block].
      *)
-    Axiom wp_case : forall sb Q, Q.(k_normal) |-- wp (Scase sb) Q.
-    Axiom wp_default : forall Q, Q.(k_normal) |-- wp Sdefault Q.
+    Axiom wp_case : forall ρ sb Q, Q.(k_normal) |-- wp ρ (Scase sb) Q.
+    Axiom wp_default : forall ρ Q, Q.(k_normal) |-- wp ρ Sdefault Q.
 
   End with_resolver.
 
